Manual/Meta/Lean.lean
@@ -50,10 +50,30 @@ def LeanBlockConfig.parse [Monad m] [MonadInfoTree m] [MonadLiftT CoreM m] [Mona
 
 open Manual.Meta.Lean.Scopes (getScopes setScopes runWithOpenDecls runWithVariables)
 
+private def abbrevFirstLine (width : Nat) (str : String) : String :=
+  let str := str.trimLeft
+  let short := str.take width |>.replace "\n" "⏎"
+  if short == str then short else short ++ "…"
+
+def LeanBlockConfig.outlineMeta : LeanBlockConfig → String
+  | {«show», error, ..} =>
+    match «show», error with
+    | some true, true | none, true => " (error)"
+    | some false, true => " (hidden, error)"
+    | some false, false => " (hidden)"
+    | _, _ => " "
+
 @[code_block_expander lean]
 def lean : CodeBlockExpander
   | args, str => do
     let config ← LeanBlockConfig.parse.run args
+
+    PointOfInterest.save (← getRef) ((config.name.map toString).getD (abbrevFirstLine 20 str.getString))
+      (kind := Lsp.SymbolKind.file)
+      (detail? := some ("Lean code" ++ config.outlineMeta))
+
+    let col? := (← getRef).getPos? |>.map (← getFileMap).utf8PosToLspPos |>.map (·.character)
+
     let origScopes ← getScopes
 
     let altStr ← parserInputString str
@@ -94,6 +114,9 @@ def lean : CodeBlockExpander
       for cmd in cmds do
         hls := hls ++ (← highlight cmd cmdState.messages.toArray cmdState.infoState.trees)
 
+      if let some col := col? then
+        hls := hls.deIndent col
+
       if config.show.getD true then
         pure #[← ``(Block.other (Block.lean $(quote hls)) #[Block.code $(quote str.getString)])]
       else
@@ -129,6 +152,90 @@ def lean : CodeBlockExpander
 where
   withNewline (str : String) := if str == "" || str.back != '\n' then str ++ "\n" else str
 
+@[code_block_expander leanTerm]
+def leanTerm : CodeBlockExpander
+  | args, str => do
+    let config ← LeanBlockConfig.parse.run args
+
+    let altStr ← parserInputString str
+
+    let col? := (← getRef).getPos? |>.map (← getFileMap).utf8PosToLspPos |>.map (·.character)
+
+    match Parser.runParserCategory (← getEnv) `term altStr (← getFileName) with
+    | .error e => throwErrorAt str e
+    | .ok stx =>
+      let (newMsgs, tree) ← do
+        let initMsgs ← Core.getMessageLog
+        try
+          Core.resetMessageLog
+          let tree' ← runWithOpenDecls <| runWithVariables fun _vars => do
+            let e ← Elab.Term.elabTerm (catchExPostpone := true) stx none
+            Term.synthesizeSyntheticMVarsNoPostponing
+            let _ ← Term.levelMVarToParam (← instantiateMVars e)
+
+            let ctx := PartialContextInfo.commandCtx {
+              env := ← getEnv, fileMap := ← getFileMap, mctx := ← getMCtx, currNamespace := ← getCurrNamespace,
+              openDecls := ← getOpenDecls, options := ← getOptions, ngen := ← getNGen
+            }
+            pure <| InfoTree.context ctx (.node (Info.ofCommandInfo ⟨`Manual.leanInline, str⟩) (← getInfoState).trees)
+          pure (← Core.getMessageLog, tree')
+        finally
+          Core.setMessageLog initMsgs
+
+      if let some name := config.name then
+        let msgs ← newMsgs.toList.mapM fun msg => do
+
+          let head := if msg.caption != "" then msg.caption ++ ":\n" else ""
+          let txt := withNewline <| head ++ (← msg.data.toString)
+
+          pure (msg.severity, txt)
+        modifyEnv (leanOutputs.modifyState · (·.insert name msgs))
+
+      pushInfoTree tree
+
+      match config.error with
+      | none =>
+        for msg in newMsgs.toArray do
+          logMessage msg
+      | some true =>
+        if newMsgs.hasErrors then
+          for msg in newMsgs.errorsToWarnings.toArray do
+            logMessage msg
+        else
+          throwErrorAt str "Error expected in code, but none occurred"
+      | some false =>
+        for msg in newMsgs.toArray do
+          logMessage msg
+        if newMsgs.hasErrors then
+          throwErrorAt str "No error expected in code, one occurred"
+
+      let hls := (← highlight stx #[] (PersistentArray.empty.push tree))
+      let hls :=
+        if let some col := col? then
+          hls.deIndent col
+        else hls
+
+      if config.show.getD true then
+        pure #[← ``(Block.other (Block.lean $(quote hls)) #[Block.code $(quote str.getString)])]
+      else
+        pure #[]
+where
+  withNewline (str : String) := if str == "" || str.back != '\n' then str ++ "\n" else str
+
+
+  modifyInfoTrees {m} [Monad m] [MonadInfoTree m] (f : PersistentArray InfoTree → PersistentArray InfoTree) : m Unit :=
+    modifyInfoState fun s => { s with trees := f s.trees }
+
+  -- TODO - consider how to upstream this
+  withInfoTreeContext {m α} [Monad m] [MonadInfoTree m] [MonadFinally m] (x : m α) (mkInfoTree : PersistentArray InfoTree → m InfoTree) : m (α × InfoTree) := do
+    let treesSaved ← getResetInfoTrees
+    MonadFinally.tryFinally' x fun _ => do
+      let st    ← getInfoState
+      let tree  ← mkInfoTree st.trees
+      modifyInfoTrees fun _ => treesSaved.push tree
+      pure tree
+
+
 @[role_expander lean]
 def leanInline : RoleExpander
   | args, inlines => do
@@ -147,7 +254,10 @@ def leanInline : RoleExpander
         try
           Core.resetMessageLog
           let tree' ← runWithOpenDecls <| runWithVariables fun _ => do
-            discard <| Elab.Term.elabTerm (catchExPostpone := true) stx none
+            let e ← Elab.Term.elabTerm (catchExPostpone := true) stx none
+            Term.synthesizeSyntheticMVarsNoPostponing
+            let _ ← Term.levelMVarToParam (← instantiateMVars e)
+
             Term.synthesizeSyntheticMVarsNoPostponing
             let ctx := PartialContextInfo.commandCtx {
               env := ← getEnv, fileMap := ← getFileMap, mctx := ← getMCtx, currNamespace := ← getCurrNamespace,
@@ -314,6 +424,11 @@ def signature : CodeBlockExpander
     | .ok stx =>
       let `(signature_spec|$[$kw]? $name:declId $sig:declSig) := stx
         | throwError m!"Didn't understand parsed signature: {indentD stx}"
+
+      PointOfInterest.save (← getRef) (toString name.raw)
+        (kind := Lsp.SymbolKind.file)
+        (detail? := some "Signature")
+
       let cmdCtx : Command.Context := {
         fileName := ← getFileName,
         fileMap := ← getFileMap,
@@ -322,8 +437,15 @@ def signature : CodeBlockExpander
         cancelTk? := none
       }
       let cmdState : Command.State := {env := ← getEnv, maxRecDepth := ← MonadRecDepth.getMaxRecDepth, infoState := ← getInfoState}
-      let ((hls, _, _, _), st') ← ((SubVerso.Examples.checkSignature name sig).run cmdCtx).run cmdState
-      setInfoState st'.infoState
+      let hls ←
+        try
+          let ((hls, _, _, _), st') ← ((SubVerso.Examples.checkSignature name sig).run cmdCtx).run cmdState
+          setInfoState st'.infoState
+          pure hls
+        catch e =>
+          let fmt ← PrettyPrinter.ppSignature (TSyntax.mk name.raw[0]).getId
+          Suggestion.saveSuggestion str (fmt.fmt.pretty 60) (fmt.fmt.pretty 30 ++ "\n")
+          throw e
 
       if «show» then
         pure #[← `(Block.other {Block.signature with data := ToJson.toJson $(quote (Highlighted.seq hls))} #[Block.code $(quote str.getString)])]
@@ -387,6 +509,11 @@ open Lean.Parser in
 def syntaxError : CodeBlockExpander
   | args, str => do
     let config ← SyntaxErrorConfig.parse.run args
+
+    PointOfInterest.save (← getRef) config.name.toString
+      (kind := Lsp.SymbolKind.file)
+      (detail? := some "Syntax error")
+
     let s := str.getString
     match runParserCategory (← getEnv) (← getOptions) config.category s with
     | .ok stx =>
@@ -555,6 +682,11 @@ defmethod Lean.NameMap.getOrSuggest [Monad m] [MonadInfoTree m] [MonadError m]
 def leanOutput : CodeBlockExpander
  | args, str => do
     let config ← LeanOutputConfig.parser.run args
+    PointOfInterest.save (← getRef) (config.name.getId.toString)
+      (kind := Lsp.SymbolKind.file)
+      (selectionRange := config.name)
+      (detail? := some ("Lean output" ++ (config.severity.map (s!" ({sevStr ·})") |>.getD "")))
+
     let msgs : List (MessageSeverity × String) ← leanOutputs.getState (← getEnv) |>.getOrSuggest config.name
 
     for (sev, txt) in msgs do
@@ -616,13 +748,18 @@ structure NameConfig where
   full : Option Name
 
 def NameConfig.parse [Monad m] [MonadError m] [MonadLiftT CoreM m] [MonadLiftT TermElabM m] : ArgParse m NameConfig :=
-  NameConfig.mk <$> ((fun _ => none) <$> .done <|> .positional `name ref <|> pure none)
+  NameConfig.mk <$> ((fun _ => none) <$> .done <|> .positional `name ref)
 where
   ref : ValDesc m (Option Name) := {
     description := m!"reference name"
     get := fun
       | .name x =>
-        some <$> liftM (runWithOpenDecls (runWithVariables fun _ => realizeGlobalConstNoOverloadWithInfo x))
+        try
+          let resolved ← liftM (runWithOpenDecls (runWithVariables fun _ => realizeGlobalConstNoOverloadWithInfo x))
+          return some resolved
+        catch
+          | .error ref e => throwErrorAt ref e
+          | _ => return none
       | other => throwError "Expected reference name, got {repr other}"
   }
 
