Manual/Language/Classes/InstanceSynth.lean
@@ -193,7 +193,7 @@ Membership.{u, v} (α : outParam (Type u)) (γ : Type v) : Type (max u v)
 ```
 
 Type class parameters can be declared as outputs by wrapping their types in the {name}`outParam` {tech}[gadget].
-When a class parameter is an output, instance synthesis will not require that it be known; in fact, any existing value is ignored completely.
+When a class parameter is an {deftech}_output parameter_, instance synthesis will not require that it be known; in fact, any existing value is ignored completely.
 The first instance that matches the input parameters is selected, and that instance's assignment of the output parameter becomes its value.
 If there was a pre-existing value, then it is compared with the assignment after synthesis is complete, and it is an error if they do not match.
 
@@ -290,7 +290,7 @@ The {lean}`OneSmaller (Option Bool) (Option Unit)` instance was selected during 
 :::
 ::::
 
-Semi-output parameters are like output parameters in that they are not required to be known prior to synthesis commencing; unlike output parameters, their values are taken into account when selecting instances.
+{deftech}_Semi-output parameters_ are like output parameters in that they are not required to be known prior to synthesis commencing; unlike output parameters, their values are taken into account when selecting instances.
 
 {docstring semiOutParam}
 
