Manual/Meta/Basic.lean
@@ -8,6 +8,7 @@ import Lean.Data.Position
 import Lean.Parser
 
 import Verso.Doc.ArgParse
+import SubVerso.Highlighting
 
 open Lean
 
@@ -19,10 +20,48 @@ def Verso.ArgParse.ValDesc.nat [Monad m] [MonadError m] : ValDesc m Nat where
     | other => throwError "Expected string, got {repr other}"
 
 
+namespace SubVerso.Highlighting
+/--
+Remove n levels of indentation from highlighted code.
+-/
+partial def Highlighted.deIndent (n : Nat) (hl : Highlighted) : Highlighted :=
+  (remove hl).run' (some n)
+where
+  remove (hl : Highlighted) : StateM (Option Nat) Highlighted := do
+    match hl with
+    | .token t =>
+      set (none : Option Nat)
+      return .token t
+    | .span i x => .span i <$> remove x
+    | .seq xs => .seq <$> xs.mapM remove
+    | .text s =>
+      let mut s' := ""
+      let mut iter := s.iter
+      while h : iter.hasNext do
+        let c := iter.curr' h
+        iter := iter.next
+        match c with
+        | '\n' =>
+          set (some n)
+        | ' ' =>
+          if let some (i + 1) ← get then
+            set (some i)
+            continue
+        | _ => set (none : Option Nat)
+        s' := s'.push c
+      return .text s'
+    | .point p s => return .point p s
+    | .tactics gs x y hl => .tactics gs x y <$> remove hl
+
+end SubVerso.Highlighting
+
 namespace Manual
 
-def parserInputString [Monad m] [MonadFileMap m] (str : TSyntax `str) : m String := do
-  let preString := (← getFileMap).source.extract 0 (str.raw.getPos?.getD 0)
+def parserInputString [Monad m] [MonadFileMap m]
+    (str : TSyntax `str) :
+    m String := do
+  let text ← getFileMap
+  let preString := text.source.extract 0 (str.raw.getPos?.getD 0)
   let mut code := ""
   let mut iter := preString.iter
   while !iter.atEnd do
@@ -31,7 +70,10 @@ def parserInputString [Monad m] [MonadFileMap m] (str : TSyntax `str) : m String
       for _ in [0:iter.curr.utf8Size] do
         code := code.push ' '
     iter := iter.next
-  code := code ++ str.getString
+  let strOriginal? : Option String := do
+    let ⟨start, stop⟩ ← str.raw.getRange?
+    text.source.extract start stop
+  code := code ++ strOriginal?.getD str.getString
   return code
 
 open Lean.Parser in
