Manual/Monads/API.lean
@@ -1,0 +1,106 @@
+/-
+Copyright (c) 2024 Lean FRO LLC. All rights reserved.
+Released under Apache 2.0 license as described in the file LICENSE.
+Author: David Thrane Christiansen
+-/
+
+import VersoManual
+
+import Manual.Meta
+
+import Lean.Parser.Command
+
+open Manual
+
+open Verso.Genre
+open Verso.Genre.Manual
+
+set_option pp.rawOnError true
+
+set_option linter.unusedVariables false
+
+#doc (Manual) "API Reference" =>
+
+In addition to the general functions described here, there are some functions that are conventionally defined as part of the API of in the namespace of each collection type:
+ * `mapM` maps a monadic function.
+ * `forM` maps a monadic function, throwing away the result.
+ * `filterM` filters using a monadic predicate, returning the values that satisfy it.
+
+
+::::example "Monadic Collection Operations"
+{name}`Array.filterM` can be used to write a filter that depends on a side effect.
+
+:::ioExample
+```ioLean
+def values := #[1, 2, 3, 5, 8]
+def main : IO Unit := do
+  let filtered ← values.filterM fun v => do
+    repeat
+      IO.println s!"Keep {v}? [y/n]"
+      let answer := (← (← IO.getStdin).getLine).trim
+      if answer == "y" then return true
+      if answer == "n" then return false
+    return false
+  IO.println "These values were kept:"
+  for v in filtered do
+    IO.println s!" * {v}"
+```
+```stdin
+y
+n
+oops
+y
+n
+y
+```
+```stdout
+Keep 1? [y/n]
+Keep 2? [y/n]
+Keep 3? [y/n]
+Keep 3? [y/n]
+Keep 5? [y/n]
+Keep 8? [y/n]
+These values were kept:
+ * 1
+ * 3
+ * 8
+```
+:::
+::::
+
+# Discarding Results
+
+The {name}`discard` function is especially useful when using an action that returns a value only for its side effects.
+
+{docstring discard}
+
+# Control Flow
+
+{docstring guard}
+
+{docstring optional}
+
+# Lifting Boolean Operations
+
+{docstring andM}
+
+{docstring orM}
+
+{docstring notM}
+
+# Kleisli Composition
+
+{deftech}_Kleisli composition_ is the composition of monadic functions, analogous to {name}`Function.comp` for ordinary functions.
+
+{docstring Bind.kleisliRight}
+
+{docstring Bind.kleisliLeft}
+
+# Re-Ordered Operations
+
+Sometimes, it can be convenient to partially apply a function to its second argument.
+These functions reverse the order of arguments, making it this easier.
+
+{docstring Functor.mapRev}
+
+{docstring Bind.bindLeft}
