Manual/Monads/Laws.lean
@@ -1,0 +1,76 @@
+/-
+Copyright (c) 2024 Lean FRO LLC. All rights reserved.
+Released under Apache 2.0 license as described in the file LICENSE.
+Author: David Thrane Christiansen
+-/
+
+import VersoManual
+
+import Manual.Meta
+
+import Lean.Parser.Command
+
+open Manual
+
+open Verso.Genre
+open Verso.Genre.Manual
+
+set_option pp.rawOnError true
+
+set_option linter.unusedVariables false
+
+#doc (Manual) "Laws" =>
+
+```lean (show := false)
+section Laws
+universe u u' v
+axiom f : Type u → Type v
+axiom m : Type u → Type v
+variable [Functor f]
+variable [Applicative f]
+variable [Monad m]
+axiom α : Type u'
+axiom β : Type u'
+axiom γ : Type u'
+axiom x : f α
+```
+
+:::keepEnv
+```lean (show := false)
+section F
+variable {f : Type u → Type v} [Functor f] {α β : Type u} {g : α → β} {h : β → γ} {x : f α}
+```
+
+Having {name Functor.map}`map`, {name Pure.pure}`pure`, {name Seq.seq}`seq`, and {name Bind.bind}`bind` operators with the appropriate types is not really sufficient to have a functor, applicative functor, or monad.
+These operators must additionally satisfy certain axioms, which are often called the {deftech}_laws_ of the type class.
+
+For a functor, the {name Functor.map}`map` operation must preserve identity and function composition. In other words, given a purported {name}`Functor` {lean}`f`, for all {lean}`x`​` : `​{lean}`f α`:
+ * {lean}`id <$> x = x`, and
+ * for all function {lean}`g` and {lean}`h`, {lean}`(h ∘ g) <$> x = h <$> g <$> x`.
+Instances that violate these assumptions can be very surprising!
+Additionally, because {lean}`Functor` includes {name Functor.mapConst}`mapConst` to enable instances to provide a more efficient implementation, a lawful functor's {name Functor.mapConst}`mapConst` should be equivalent to its default implementation.
+
+The Lean standard library does not require profs of these properties in every instance of {name}`Functor`.
+Nonetheless, if an instance violates them, then it should be considered a bug.
+When proofs of these properties are necessary, an instance implicit parameter of type {lean}`LawfulFunctor f` can be used.
+The {name}`LawfulFunctor` class includes the necessary proofs.
+
+{docstring LawfulFunctor}
+
+```lean (show := false)
+end F
+```
+:::
+
+
+
+
+In addition to proving that the potentially-optimized {name}`SeqLeft.seqLeft` and {name}`SeqRight.seqRight` operations are equivalent to their default implementations, Applicative functors {lean}`f` must satisfy four laws.
+
+{docstring LawfulApplicative}
+
+The {deftech}[monad laws] specify that {name}`pure` followed by {name}`bind` should be equivalent to function application (that is, {name}`pure` has no effects), that {name}`bind` followed by {name}`pure` around a function application is equivalent to {name Functor.map}`map`, and that {name}`bind` is associative.
+
+{docstring LawfulMonad}
+
+{docstring LawfulMonad.mk'}
