Manual/Monads/Syntax.lean
@@ -1,0 +1,808 @@
+/-
+Copyright (c) 2024 Lean FRO LLC. All rights reserved.
+Released under Apache 2.0 license as described in the file LICENSE.
+Author: David Thrane Christiansen
+-/
+
+import VersoManual
+
+import Manual.Meta
+
+import Lean.Parser.Command
+
+open Manual
+
+open Verso.Genre
+open Verso.Genre.Manual
+
+set_option pp.rawOnError true
+
+set_option linter.unusedVariables false
+-- set_option trace.SubVerso.Highlighting.Code true
+
+#doc (Manual) "Syntax" =>
+
+Lean supports programming with functors, applicative functors, and monads via special syntax:
+ * Infix operators are provided for the most common operations.
+ * An embedded language called {tech}[{keywordOf Lean.Parser.Term.do}`do`-notation] allows the use of imperative syntax when writing programs in a monad.
+
+# Infix Operators
+
+Infix operators are primarily useful in smaller expressions, or when there is no {lean}`Monad` instance.
+
+## Functors
+
+```lean (show := false)
+section FOps
+variable {f : Type u → Type v} [Functor f] {α β : Type u} {g : α → β} {x : f α}
+```
+There are two infix operators for {name}`Functor.map`.
+
+:::syntax term (title := "Functor Operators")
+{lean}`g <$> x` is short for {lean}`Functor.map g x`.
+```grammar
+$_ <$> $_
+```
+
+{lean}`x <&> g` is short for {lean}`Functor.map g x`.
+```grammar
+$_ <&> $_
+```
+:::
+
+```lean (show := false)
+example : g <$> x = Functor.map g x := by rfl
+example : x <&> g = Functor.map g x := by rfl
+end FOps
+```
+
+## Applicative Functors
+
+```lean (show := false)
+section AOps
+variable {f : Type u → Type v} [Applicative f] [Alternative f] {α β : Type u} {g : f (α → β)} {x e1 e e' : f α} {e2 : f β}
+```
+
+:::syntax term (title := "Applicative Operators")
+{lean}`g <*> x` is short for {lean}`Seq.seq g (fun () => x)`.
+The function is inserted to delay evaluation because control might not reach the argument.
+```grammar
+$_ <*> $_
+```
+
+{lean}`e1 *> e2` is short for {lean}`SeqRight.seqRight e1 (fun () => e2)`.
+```grammar
+$_ *> $_
+```
+
+{lean}`e1 <* e2` is short for {lean}`SeqLeft.seqLeft e1 (fun () => e2)`.
+```grammar
+$_ <* $_
+```
+:::
+
+Many applicative functors also support failure and recovery via the {name}`Alternative` type class.
+This class also has an infix operator.
+
+:::syntax term (title := "Alternative Operators")
+{lean}`e <|> e'` is short for {lean}`OrElse.orElse e (fun () => e')`.
+The function is inserted to delay evaluation because control might not reach the argument.
+```grammar
+$_ <|> $_
+```
+:::
+
+
+```lean (show := false)
+example : g <*> x = Seq.seq g (fun () => x) := by rfl
+example : e1 *> e2 = SeqRight.seqRight e1 (fun () => e2) := by rfl
+example : e1 <* e2 = SeqLeft.seqLeft e1 (fun () => e2) := by rfl
+example : (e <|> e') = (OrElse.orElse e (fun () => e')) := by rfl
+end AOps
+```
+
+:::::keepEnv
+```lean
+structure User where
+  name : String
+  favoriteNat : Nat
+def main : IO Unit := pure ()
+```
+::::example "Infix `Functor` and `Applicative` Operators"
+A common functional programming idiom is to use a pure function in some context with effects by applying it via {name}`Functor.map` and {name}`Seq.seq`.
+The function is applied to its sequence of arguments using `<$>`, and the arguments are separated by `<*>`.
+
+In this example, the constructor {name}`User.mk` is applied via this idiom in the body of {lean}`main`.
+:::ioExample
+```ioLean
+def getName : IO String := do
+  IO.println "What is your name?"
+  return (← (← IO.getStdin).getLine).trimRight
+
+partial def getFavoriteNat : IO Nat := do
+  IO.println "What is your favorite natural number?"
+  let line ← (← IO.getStdin).getLine
+  if let some n := line.trim.toNat? then
+    return n
+  else
+    IO.println "Let's try again."
+    getFavoriteNat
+
+structure User where
+  name : String
+  favoriteNat : Nat
+deriving Repr
+
+def main : IO Unit := do
+  let user ← User.mk <$> getName <*> getFavoriteNat
+  IO.println (repr user)
+```
+When run with this input:
+```stdin
+A. Lean User
+None
+42
+```
+it produces this output:
+```stdout
+What is your name?
+What is your favorite natural number?
+Let's try again.
+What is your favorite natural number?
+{ name := "A. Lean User", favoriteNat := 42 }
+```
+:::
+
+::::
+:::::
+
+## Monads
+
+Monads are primarily used via {tech}[{keywordOf Lean.Parser.Term.do}`do`-notation].
+However, it can sometimes be convenient to describe monadic computations via operators.
+
+```lean (show := false)
+section MOps
+variable {m : Type u → Type v} [Monad m] {α β : Type u} {act : m α} {f : α → m β} {g : β → m γ}
+```
+
+:::syntax term (title := "Monad Operators")
+
+{lean}`act >>= f` is syntax for {lean}`Bind.bind act f`.
+```grammar
+$_ >>= $_
+```
+
+Similarly, the reversed operator {lean}`f =<< act` is syntax for {lean}`Bind.bind act f`.
+```grammar
+$_ =<< $_
+```
+
+The Kleisli composition operators {name}`Bind.kleisliRight` and {name}`Bind.kleisliLeft` also have infix operators.
+```grammar
+$_ >=> $_
+```
+```grammar
+$_ <=< $_
+```
+
+:::
+
+```lean (show := false)
+example : act >>= f = Bind.bind act f := by rfl
+example : f =<< act = Bind.bind act f := rfl
+example : f >=> g = Bind.kleisliRight f g := by rfl
+example : g <=< f = Bind.kleisliLeft g f := by rfl
+end MOps
+```
+
+
+# `do`-Notation
+%%%
+tag := "do-notation"
+%%%
+
+Monads are primarily used via {deftech}[{keywordOf Lean.Parser.Term.do}`do`-notation], which is an embedded language for programming in an imperative style.
+It provides familiar syntax for sequencing effectful operations, early return, local mutable variables, loops, and exception handling.
+All of these features are translated to the operations of the {lean}`Monad` type class, with a few of them requiring addition instances of classes such as {lean}`ForIn` that specify iteration over containers.
+A {keywordOf Lean.Parser.Term.do}`do` term consists of the keyword {keywordOf Lean.Parser.Term.do}`do` followed by a sequence of {deftech}_{keywordOf Lean.Parser.Term.do}`do` items_.
+
+:::syntax term
+```grammar
+do $stmt*
+```
+The items in a {keywordOf Lean.Parser.Term.do}`do` may be separated by semicolons; otherwise, each should be on its own line and they should have equal indentation.
+:::
+
+```lean (show := false)
+section
+variable {m : Type → Type} [Monad m] {α β γ: Type} {e1 : m Unit} {e : β} {es : m α}
+```
+
+## Sequential Computations
+
+One form of {tech}[{keywordOf Lean.Parser.Term.do}`do` item] is a term.
+
+:::syntax Lean.Parser.Term.doSeqItem
+```grammar
+$e:term
+```
+:::
+
+
+A term followed by a sequence of items is translated to a use {name}`bind`; in particular, {lean}`do e1; es` is translated to {lean}`e1 >>= fun () => do es`.
+
+
+:::table (header := true)
+* ignored
+  * {keywordOf Lean.Parser.Term.do}`do` Item
+  * Desugaring
+* ignored
+  * ```leanTerm
+    do
+    e1
+    es
+    ```
+  * ```leanTerm
+    e1 >>= fun () => do es
+    ```
+:::
+
+```lean (show := false) (keep := false)
+def ex1a := do e1; es
+def ex1b := e1 >>= fun () => do es
+example : @ex1a = @ex1b := by rfl
+```
+
+The result of the term's computation may also be named, allowing it to be used in subsequent steps.
+This is done using {keywordOf Lean.Parser.Term.doLet}`let`.
+
+```lean (show := false)
+section
+variable {e1 : m β} {e1? : m (Option β)} {fallback : m α} {e2 : m γ} {f : β → γ → m Unit} {g : γ → α} {h : β → m γ}
+```
+
+:::syntax Lean.Parser.Term.doSeqItem
+There are two forms of monadic {keywordOf Lean.Parser.Term.doLet}`let`-binding in a {keywordOf Lean.Parser.Term.do}`do` block.
+The first binds an identifier to the result, with an optional type annotation:
+```grammar
+let $x:ident$[:$e]? ← $e:term
+```
+The second binds a pattern to the result.
+The fallback clause, beginning with `|`, specifies the behavior when the pattern does not match the result.
+```grammar
+let $x:term ← $e:term
+  $[| $e]?
+```
+:::
+This syntax is also translated to a use of {name}`bind`.
+{lean}`do let x ← e1; es` is translated to {lean}`e1 >>= fun x => do es`, and fallback clauses are translated to default pattern matches.
+{keywordOf Lean.Parser.Term.doLet}`let` may also be used with the standard definition syntax `:=` instead of `←`.
+This indicates a pure, rather than monadic, definition:
+:::syntax Lean.Parser.Term.doSeqItem
+```grammar
+let v := $e:term
+```
+:::
+{lean}`do let x := e; es` is translated to {lean}`let x := e; do es`.
+
+:::table (header := true)
+* ignored
+  * {keywordOf Lean.Parser.Term.do}`do` Item
+  * Desugaring
+* ignored
+  * ```leanTerm
+    do
+    let x ← e1
+    es
+    ```
+  * ```leanTerm
+    e1 >>= fun x =>
+      do es
+    ```
+* ignored
+  * ```leanTerm
+    do
+    let some x ← e1?
+      | fallback
+    es
+    ```
+  * ```leanTerm
+    e1? >>= fun
+      | some x => do
+        es
+      | _ => fallback
+    ```
+* ignored
+  * ```leanTerm
+    do
+    let x := e
+    es
+    ```
+  * ```leanTerm
+    let x := e
+    do es
+    ```
+:::
+
+```lean (show := false) (keep := false)
+-- Test desugarings
+def ex1a := do
+    let x ← e1
+    es
+def ex1b :=
+    e1 >>= fun x =>
+      do es
+example : @ex1a = @ex1b := by rfl
+
+
+def ex2a :=
+    do
+    let some x ← e1?
+      | fallback
+    es
+
+def ex2b :=
+    e1? >>= fun
+      | some x => do
+        es
+      | _ => fallback
+example : @ex2a = @ex2b := by rfl
+
+def ex3a :=
+    do
+    let x := e
+    es
+def ex3b :=
+    let x := e
+    do es
+example : @ex3a = @ex3b := by rfl
+```
+Within a {keywordOf Lean.Parser.Term.do}`do` block, `←` may be used as a prefix operator.
+The expression to which it is applied is replaced with a fresh variable, which is bound using {name}`bind` just before the current step.
+This allows monadic effects to be used in positions that otherwise might expect a pure value, while still maintaining the distinction between _describing_ an effectful computation and actually _executing_ its effects.
+Multiple occurrences of `←` are processed from left to right, inside to outside.
+
+::::figure "Example Nested Action Desugarings"
+:::table (header := true)
+* ignored
+  * Example {keywordOf Lean.Parser.Term.do}`do` Item
+  * Desugaring
+* ignored
+  * ```leanTerm
+    do
+    f (← e1) (← e2)
+    es
+    ```
+  * ```leanTerm
+    do
+    let x ← e1
+    let y ← e2
+    f x y
+    es
+    ```
+* ignored
+  * ```leanTerm
+    do
+    let x := g (← h (← e1))
+    es
+    ```
+  * ```leanTerm
+    do
+    let y ← e1
+    let z ← h y
+    let x := g z
+    es
+    ```
+:::
+::::
+
+```lean (show := false) (keep := false)
+-- Test desugarings
+def ex1a := do
+  f (← e1) (← e2)
+  es
+def ex1b := do
+  let x ← e1
+  let y ← e2
+  f x y
+  es
+example : @ex1a = @ex1b := by rfl
+def ex2a := do
+  let x := g (← h (← e1))
+  es
+def ex2b := do
+  let y ← e1
+  let z ← h y
+  let x := g z
+  es
+example : @ex2a = @ex2b := by rfl
+```
+
+In addition to convenient support for sequential computations with data dependencies, {keywordOf Lean.Parser.Term.do}`do`-notation also supports the local addition of a variety of effects, including early return, local mutable state, and loops with early termination.
+These effects are implemented via transformations of the entire {keywordOf Lean.Parser.Term.do}`do` block in a manner akin to {tech}[monad transformers], rather than via a local desugaring.
+
+## Early Return
+
+Early return terminates a computation immediately with a given value.
+The value is returned from the closest containing {keywordOf Lean.Parser.Term.do}`do` block; however, this may not be the closest `do` keyword.
+The rules for determining the extent of a {keywordOf Lean.Parser.Term.do}`do` block are described {ref "closest-do-block"}[in their own section].
+
+:::syntax Lean.Parser.Term.doSeqItem
+```grammar
+return $e
+```
+
+```grammar
+return
+```
+:::
+
+Not all monads include early return.
+Thus, when a {keywordOf Lean.Parser.Term.do}`do` block contains {keywordOf Lean.Parser.Term.doReturn}`return`, the code needs to be rewritten to simulate the effect.
+A program that uses early return to compute a value of type {lean}`α` in a monad {lean}`m` can be thought of as a program in the monad {lean}`ExceptT α m α`: early-returned values take the exception pathway, while ordinary returns do not.
+Then, an outer handler can return the value from either code paths.
+Internally, the {keywordOf Lean.Parser.Term.do}`do` elaborator performs a translation very much like this one.
+
+On its own, {keywordOf Lean.Parser.Term.doReturn}`return` is short for {keywordOf Lean.Parser.Term.doReturn}`return`​` `​{lean}`()`.
+
+## Local Mutable State
+
+Local mutable state is mutable state that cannot escape the {keywordOf Lean.Parser.Term.do}`do` block in which it is defined.
+The {keywordOf Lean.Parser.Term.doLet}`let mut` binder introduces a locally-mutable binding.
+:::syntax Lean.Parser.Term.doSeqItem
+Mutable bindings may be initialized either with pure computations or with monadic computations:
+```grammar
+let mut $x := $e
+```
+```grammar
+let mut $x ← $e
+```
+
+Similarly, they can be mutated either with pure values or the results of monad computations:
+```grammar (of := Lean.Parser.Term.doReassign)
+$x:ident$[: $_]?  := $e:term
+```
+```grammar (of := Lean.Parser.Term.doReassign)
+$x:term$[: $_]? := $e:term
+```
+```grammar (of := Lean.Parser.Term.doReassignArrow)
+$x:ident$[: $_]? ← $e:term
+```
+```grammar (of := Lean.Parser.Term.doReassignArrow)
+$x:term ← $e:term
+  $[| $e]?
+```
+:::
+
+These locally-mutable bindings are less powerful than a {tech}[state monad] because they are not mutable outside their lexical scope; this also makes them easier to reason about.
+When {keywordOf Lean.Parser.Term.do}`do` blocks contain mutable bindings, the {keywordOf Lean.Parser.Term.do}`do` elaborator transforms the expression similarly to the way that {lean}`StateT` would, constructing a new monad and initializing it with the correct values.
+
+## Control Structures
+
+There are {keywordOf Lean.Parser.Term.do}`do` items that correspond to most of Lean's term-level control structures.
+When they occur as a step in a {keywordOf Lean.Parser.Term.do}`do` block, they are interpreted as {keywordOf Lean.Parser.Term.do}`do` items rather than terms.
+Each branch of the control structures is a sequence of {keywordOf Lean.Parser.Term.do}`do` items, rather than a term, and some of them are more syntactically flexible than their corresponding terms.
+
+:::syntax Lean.Parser.Term.doSeqItem
+In a {keywordOf Lean.Parser.Term.do}`do` block, {keywordOf Lean.Parser.Term.doIf}`if` statements may omit their {keywordOf Lean.Parser.Term.doIf}`else` branch.
+Omitting an {keywordOf Lean.Parser.Term.doIf}`else` branch is equivalent to using {name}`pure`{lean}` ()` as the contents of the branch.
+```grammar
+if $[$h :]? $e then
+  $e*
+$[else
+  $_*]?
+```
+:::
+
+Syntactically, the {keywordOf Lean.Parser.Term.doIf}`then` branch cannot be omitted.
+For these cases, {keywordOf Lean.Parser.Term.doUnless}`unless` only executes its body when the condition is false.
+The {keywordOf Lean.Parser.Term.do}`do` in {keywordOf Lean.Parser.Term.doUnless}`unless` is part of its syntax and does not induce a nested {keywordOf Lean.Parser.Term.do}`do` block.
+:::syntax Lean.Parser.Term.doSeqItem
+```grammar
+unless $e do
+  $e*
+```
+:::
+
+
+When {keywordOf Lean.Parser.Term.doMatch}`match` is used in a {keywordOf Lean.Parser.Term.do}`do` block, each branch is considered to be part of the same block.
+Otherwise, it is equivalent to the {keywordOf Lean.Parser.Term.match}`match` term.
+:::syntax Lean.Parser.Term.doSeqItem
+```grammar
+match $[$[$h :]? $e],* with
+  $[| $t,* => $e*]*
+```
+:::
+
+
+## Iteration
+
+Within a {keywordOf Lean.Parser.Term.do}`do` block, {keywordOf Lean.Parser.Term.doFor}`for`​`…`​{keywordOf Lean.Parser.Term.doFor}`in` loops allow iteration over a data structure.
+The body of the loop is part of the containing {keywordOf Lean.Parser.Term.do}`do` block, so local effects such as early return and mutable variables may be used.
+
+:::syntax Lean.Parser.Term.doSeqItem
+```grammar
+for $[$[$h :]? $x in $y],* do
+  $e*
+```
+:::
+
+A {keywordOf Lean.Parser.Term.doFor}`for`​`…`​{keywordOf Lean.Parser.Term.doFor}`in` loop requires at least one clause that specifies the iteration to be performed, which consists of an optional membership proof name followed by a colon (`:`), a pattern to bind, the keyword {keywordOf Lean.Parser.Term.doFor}`in`, and a collection term.
+The pattern, which may just be an {tech}[identifier], must match any element of the collection; patterns in this position cannot be used as implicit filters.
+Further clauses may be provided by separating them with commas.
+Each collection is iterated over at the same time, and iteration stops when any of the collections runs out of elements.
+
+:::example "Iteration Over Multiple Collections"
+When iterating over multiple collections, iteration stops when any of the collections runs out of elements.
+```lean (name := earlyStop)
+#eval Id.run do
+  let mut v := #[]
+  for x in [0:43], y in ['a', 'b'] do
+    v := v.push (x, y)
+  return v
+```
+```leanOutput earlyStop
+#[(0, 'a'), (1, 'b')]
+```
+:::
+
+::::keepEnv
+:::example "Iteration over Array Indices with {keywordOf Lean.Parser.Term.doFor}`for`"
+
+When iterating over the valid indices for an array with {keywordOf Lean.Parser.Term.doFor}`for`, naming the membership proof allows the tactic that searches for proofs that array indices are in bounds to succeed.
+```lean (keep := false)
+def satisfyingIndices (p : α → Prop) [DecidablePred p] (xs : Array α) : Array Nat := Id.run do
+  let mut out := #[]
+  for h : i in [0:xs.size] do
+    if p xs[i] then out := out.push i
+  return out
+```
+
+Omitting the hypothesis name causes the array lookup to fail, because no proof is available in the context that the iteration variable is within the specified range.
+
+```lean (keep := false) (show := false)
+-- test it
+/--
+error: failed to prove index is valid, possible solutions:
+  - Use `have`-expressions to prove the index is valid
+  - Use `a[i]!` notation instead, runtime check is performed, and 'Panic' error message is produced if index is not valid
+  - Use `a[i]?` notation instead, result is an `Option` type
+  - Use `a[i]'h` notation instead, where `h` is a proof that index is valid
+m : Type → Type
+inst✝¹ : Monad m
+α β γ : Type
+e1✝ : m Unit
+e : β
+es : m α
+e1 : m β
+e1? : m (Option β)
+fallback : m α
+e2 : m γ
+f : β → γ → m Unit
+g : γ → α
+h : β → m γ
+p : α → Prop
+inst✝ : DecidablePred p
+xs : Array α
+out✝ : Array Nat := #[]
+col✝ : Std.Range := { start := 0, stop := xs.size, step := 1 }
+i : Nat
+r✝ : Array Nat
+out : Array Nat := r✝
+⊢ i < xs.size
+-/
+#guard_msgs in
+def satisfyingIndices (p : α → Prop) [DecidablePred p] (xs : Array α) : Array Nat := Id.run do
+  let mut out := #[]
+  for i in [0:xs.size] do
+    if p xs[i] then out := out.push i
+  return out
+```
+:::
+::::
+
+The body of a {keywordOf Lean.doElemWhile_Do_}`while` loop is repeated while the condition remains true.
+It is possible to write infinite loops using them in functions that are not marked {keywordOf Lean.Parser.Command.declaration}`partial`.
+This is because the {keywordOf Lean.Parser.Command.declaration}`partial` modifier only applies to non-termination or infinite regress induced by the function being defined, and not by those that it calls.
+The translation of {keywordOf Lean.doElemWhile_Do_}`while` loops relies on a separate helper.
+
+:::syntax Lean.Parser.Term.doSeqItem
+```grammar
+while $e do
+  $e*
+```
+```grammar
+while $h : $e do
+  $e*
+```
+:::
+
+The body of a {keywordOf Lean.doElemRepeat_}`repeat` loop is repeated until a {keywordOf Lean.Parser.Term.doBreak}`break` statement is executed.
+Just like {keywordOf Lean.doElemWhile_Do_}`while` loops, these loops can be used in functions that are not marked {keywordOf Lean.Parser.Command.declaration}`partial`.
+
+:::syntax Lean.Parser.Term.doSeqItem
+```grammar
+repeat
+  $e*
+```
+:::
+
+The {keywordOf Lean.Parser.Term.doContinue}`continue` statement skips the rest of the body of the closest enclosing {keywordOf Lean.doElemRepeat_}`repeat`, {keywordOf Lean.doElemWhile_Do_}`while`, or {keywordOf Lean.Parser.Term.doFor}`for` loop, moving on to the next iteration.
+The {keywordOf Lean.Parser.Term.doBreak}`break` statement terminates the closest enclosing {keywordOf Lean.doElemRepeat_}`repeat`, {keywordOf Lean.doElemWhile_Do_}`while`, or {keywordOf Lean.Parser.Term.doFor}`for` loop, stopping iteration.
+
+:::syntax Lean.Parser.Term.doSeqItem
+```grammar
+continue
+```
+```grammar
+break
+```
+:::
+
+In addition to {keywordOf Lean.Parser.Term.doBreak}`break`, loops can always be terminated by effects in the current monad.
+Throwing an exception from a loop terminates the loop.
+
+:::example "Terminating Loops in the {lean}`Option` Monad"
+The {name}`failure` method from the {name}`Alternative` class can be used to terminate an otherwise-infinite loop in the {name}`Option` monad.
+
+```lean (name := natBreak)
+#eval show Option Nat from do
+  let mut i := 0
+  repeat
+    if i > 1000 then failure
+    else i := 2 * (i + 1)
+  return i
+```
+```leanOutput natBreak
+none
+```
+:::
+
+## Identifying `do` Blocks
+%%%
+tag := "closest-do-block"
+%%%
+
+Many features of {keywordOf Lean.Parser.Term.do}`do`-notation have an effect on the {deftech}[current {keywordOf Lean.Parser.Term.do}`do` block].
+In particular, early return aborts the current block, causing it to evaluate to the returned value, and mutable bindings can only be mutated in the block in which they are defined.
+Understanding these features requires a precise definition of what it means to be in the “same” block.
+
+Empirically, this can be checked using the Lean language server.
+When the cursor is on a {keywordOf Lean.Parser.Term.doReturn}`return` statement, the corresponding {keywordOf Lean.Parser.Term.do}`do` keyword is highlighted.
+Attempting to mutate a mutable binding outside of the same {keywordOf Lean.Parser.Term.do}`do` block results in an error message.
+
+:::figure "Highlighting {keywordOf Lean.Parser.Term.do}`do`"
+
+![Highlighting do from return](/static/screenshots/do-return-hl-1.png)
+
+![Highlighting do from return with errors](/static/screenshots/do-return-hl-2.png)
+:::
+
+The rules are as follows:
+ * Each item immediately nested under the {keywordOf Lean.Parser.Term.do}`do` keyword that begins a block belongs to that block.
+ * Each item immediately nested under the {keywordOf Lean.Parser.Term.do}`do` keyword that is an item in a containing {keywordOf Lean.Parser.Term.do}`do` block belongs to the outer block.
+ * Items in the branches of an {keywordOf Lean.Parser.Term.doIf}`if`, {keywordOf Lean.Parser.Term.doMatch}`match`, or {keywordOf Lean.Parser.Term.doUnless}`unless` item belong to the same {keywordOf Lean.Parser.Term.do}`do` block as the control structure that contains them. The {keywordOf Lean.Parser.Term.doUnless}`do` keyword that is part of the syntax of {keywordOf Lean.Parser.Term.doUnless}`unless` does not introduce a new {keywordOf Lean.Parser.Term.do}`do` block.
+ * Items in the body of {keywordOf Lean.doElemRepeat_}`repeat`, {keywordOf Lean.doElemWhile_Do_}`while`, and {keywordOf Lean.Parser.Term.doFor}`for` belong to the same {keywordOf Lean.Parser.Term.do}`do` block as the loop  that contains them. The {keywordOf Lean.Parser.Term.doFor}`do` keyword that is part of the syntax of {keywordOf Lean.doElemWhile_Do_}`while` and {keywordOf Lean.Parser.Term.doFor}`for` does not introduce a new {keywordOf Lean.Parser.Term.do}`do` block.
+
+```lean (show := false)
+-- Test nested `do` rules
+
+/-- info: ((), 6) -/
+#guard_msgs in
+#eval (·.run 0) <| show StateM Nat Unit from do
+  set 5
+  do
+    set 6
+    return
+
+/-- error: must be last element in a `do` sequence -/
+#guard_msgs in
+#eval (·.run 0) <| show StateM Nat Unit from do
+  set 5
+  do
+    set 6
+    return
+  set 7
+  return
+
+/-- info: ((), 6) -/
+#guard_msgs in
+#eval (·.run 0) <| show StateM Nat Unit from do
+  set 5
+  if true then
+    set 6
+    do return
+  set 7
+  return
+```
+
+::::keepEnv
+:::example "Nested `do` and Branches"
+The following example outputs {lean}`6` rather than {lean}`7`:
+```lean (name := nestedDo)
+def test : StateM Nat Unit := do
+  set 5
+  if true then
+    set 6
+    do return
+  set 7
+  return
+
+#eval test.run 0
+```
+```leanOutput nestedDo
+((), 6)
+```
+
+This is because the {keywordOf Lean.Parser.Term.doReturn}`return` statement under the {keywordOf Lean.Parser.Term.doIf}`if` belongs to the same {keywordOf Lean.Parser.Term.do}`do` as its immediate parent, which itself belongs to the same {keywordOf Lean.Parser.Term.do}`do` as the {keywordOf Lean.Parser.Term.doIf}`if`.
+If {keywordOf Lean.Parser.Term.do}`do` blocks that occurred as items in other {keywordOf Lean.Parser.Term.do}`do` blocks instead created new blocks, then the example would output {lean}`7`.
+:::
+::::
+
+```lean (show := false)
+end
+```
+
+```lean (show := false)
+-- tests for this section
+set_option pp.all true
+
+/--
+info: @Bind.bind.{0, 0} m (@Monad.toBind.{0, 0} m inst✝) Unit α e1 fun (x : PUnit.{1}) => es : m α
+-/
+#guard_msgs in
+#check do e1; es
+
+section
+variable {e1 : m β}
+/-- info: @Bind.bind.{0, 0} m (@Monad.toBind.{0, 0} m inst✝) β α e1 fun (x : β) => es : m α -/
+#guard_msgs in
+#check do let x ← e1; es
+end
+
+/--
+info: let x : β := e;
+es : m α
+-/
+#guard_msgs in
+#check do let x := e; es
+
+variable {e1 : m β} {e2 : m γ} {f : β → γ → m Unit} {g : γ → α} {h : β → m γ}
+
+/--
+info: @Bind.bind.{0, 0} m (@Monad.toBind.{0, 0} m inst✝) β α e1 fun (__do_lift : β) =>
+  @Bind.bind.{0, 0} m (@Monad.toBind.{0, 0} m inst✝) γ α e2 fun (__do_lift_1 : γ) =>
+    @Bind.bind.{0, 0} m (@Monad.toBind.{0, 0} m inst✝) Unit α (f __do_lift __do_lift_1) fun (x : PUnit.{1}) => es : m α
+-/
+#guard_msgs in
+#check do f (← e1) (← e2); es
+
+/--
+info: @Bind.bind.{0, 0} m (@Monad.toBind.{0, 0} m inst✝) β α e1 fun (__do_lift : β) =>
+  @Bind.bind.{0, 0} m (@Monad.toBind.{0, 0} m inst✝) γ α (h __do_lift) fun (__do_lift : γ) =>
+    let x : α := g __do_lift;
+    es : m α
+-/
+#guard_msgs in
+#check do let x := g (← h (← e1)); es
+
+end
+
+
+```
+
+## Type Classes for Iteration
+
+To be used with {keywordOf Lean.Parser.Term.doFor}`for` loops without membership proofs, collections must implement the {name}`ForIn` type class.
+Implementing {lean}`ForIn'` additionally allows the use of {keywordOf Lean.Parser.Term.doFor}`for` loops with membership proofs.
+
+{docstring ForIn}
+
+{docstring ForIn'}
+
+{docstring ForInStep}
+
+{docstring ForM}
+
+{docstring ForM.forIn}
