Manual/Monads/Zoo.lean
@@ -1,0 +1,363 @@
+/-
+Copyright (c) 2024 Lean FRO LLC. All rights reserved.
+Released under Apache 2.0 license as described in the file LICENSE.
+Author: David Thrane Christiansen
+-/
+
+import Manual.Monads.Zoo.State
+import Manual.Monads.Zoo.Reader
+import Manual.Monads.Zoo.Except
+import Manual.Monads.Zoo.Combined
+import Manual.Monads.Zoo.Id
+import Manual.Monads.Zoo.Option
+
+/-
+Copyright (c) 2024 Lean FRO LLC. All rights reserved.
+Released under Apache 2.0 license as described in the file LICENSE.
+Author: David Thrane Christiansen
+-/
+
+import VersoManual
+
+import Manual.Meta
+
+import Lean.Parser.Command
+
+open Manual
+
+open Verso.Genre
+open Verso.Genre.Manual
+
+set_option pp.rawOnError true
+
+set_option linter.unusedVariables false
+-- set_option trace.SubVerso.Highlighting.Code true
+
+#doc (Manual) "Varieties of Monads" =>
+
+
+The {lean}`IO` monad has many, many effects, and is used for writing programs that need to interact with the world.
+It is described in {ref "io"}[its own section].
+Programs that use {lean}`IO` are essentially black boxes: they are typically not particularly amenable to verification.
+
+Many algorithms are easiest to express with a much smaller set of effects.
+These effects can often be simulated; for example, mutable state can be simulated by passing around a tuple that contains both the program's value and the state.
+These simulated effects are easier to reason formally about, because they are defined using ordinary code rather than new language primitives.
+
+The standard library provides abstractions for working with commonly-used effects.
+Many frequently-used effects fall into a small number of categories:
+
+: {deftech}[State monads] have mutable state
+
+  Computations that have access to some data that may be modified by other parts of the computation use _mutable state_.
+  State can be implemented in a variety of ways, described in the section on {ref "state-monads"}[state monads] and captured in the {name}`MonadState` type class.
+
+: {deftech}[Reader monads] are parameterized computations
+
+  Computations that can read the value of some parameter provided by a context exist in most programming languages, but many languages that feature state and exceptions as first-class features do not have built-in facilities for defining new parameterized computations.
+  Typically, these computations are provided with a parameter value when invoked, and sometimes they can locally override it.
+  Parameter values have _dynamic extent_: the value provided most recently in the call stack is the one that is used.
+  They can be simulated by passing a value unchanged through a sequence of function calls; however, this technique can make code harder to read and introduces a risk that the values may be passed incorrectly to further calls by mistake.
+  They can also be simulated using mutable state with a careful discipline surrounding the modification of the state.
+  Monads that maintain a parameter, potentially allowing it to be overridden in a section of the call stack, are called _reader monads_.
+  Reader monads are captured in the {lean}`MonadReader` type class.
+  Additionally, reader monads that allow the parameter value to be locally overridden are captured in the {lean}`MonadWithReader` type class.
+
+: {deftech}[Exception monads] have exceptions
+
+  Computations that may terminate early with an exceptional value use _exceptions_.
+  They are typically modeled with a sum type that has a constructor for ordinary termination and a constructor for early termination with errors.
+  Exception monads are described in the section on {ref "exception-monads"}[exception monads], and captured in the {name}`MonadExcept` type class.
+
+
+# Monad Type Classes
+
+Using type classes like {lean}`MonadState` and {lean}`MonadExcept` allow client code to be polymorphic with respect to monads.
+Together with automatic lifting, this allows programs to be re-usable in many different monads and makes them more robust to refactoring.
+
+It's important to be aware that effects in a monad may not interact in only one way.
+For example, a monad with state and exceptions may or may not roll back state changes when an exception is thrown.
+If this matters for the correctness of a function, then it should use a more specific signature.
+
+::::keepEnv
+:::example "Effect Ordering"
+The function {name}`sumNonFives` adds the contents of a list using a state monad, terminating early if it encounters a {lean}`5`.
+```lean
+def sumNonFives {m}
+    [Monad m] [MonadState Nat m] [MonadExcept String m]
+    (xs : List Nat) :
+    m Unit := do
+  for x in xs do
+    if x == 5 then
+      throw "Five was encountered"
+    else
+      modify (· + x)
+```
+
+Running it in one monad returns the state at the time that {lean}`5` was encountered:
+```lean (name := exSt)
+#eval
+  sumNonFives (m := ExceptT String (StateM Nat))
+    [1, 2, 3, 4, 5, 6] |>.run |>.run 0
+```
+```leanOutput exSt
+(Except.error "Five was encountered", 10)
+```
+
+In another, the state is discarded:
+```lean (name := stEx)
+#eval
+  sumNonFives (m := StateT Nat (Except String))
+    [1, 2, 3, 4, 5, 6] |>.run 0
+```
+```leanOutput stEx
+Except.error "Five was encountered"
+```
+
+In the second case, an exception handler would roll back the state to its value at the start of the {keywordOf Lean.Parser.Term.termTry}`try`.
+The following function is thus incorrect:
+```lean
+/-- Computes the sum of the non-5 prefix of a list. -/
+def sumUntilFive {m}
+    [Monad m] [MonadState Nat m] [MonadExcept String m]
+    (xs : List Nat) :
+    m Nat := do
+  MonadState.set 0
+  try
+    sumNonFives xs
+  catch _ =>
+    pure ()
+  get
+```
+
+In one monad, the answer is correct:
+```lean (name := exSt2)
+#eval
+  sumUntilFive (m := ExceptT String (StateM Nat))
+    [1, 2, 3, 4, 5, 6] |>.run |>.run' 0
+```
+```leanOutput exSt2
+Except.ok 10
+```
+
+In the other, it is not:
+```lean (name := stEx2)
+#eval
+  sumUntilFive (m := StateT Nat (Except String))
+    [1, 2, 3, 4, 5, 6] |>.run' 0
+```
+```leanOutput stEx2
+Except.ok 0
+```
+:::
+::::
+
+A single monad may support multiple version of the same effect.
+For example, there might be a mutable {lean}`Nat` and a mutable {lean}`String` or two separate reader parameters.
+As long as they have different types, it should be convenient to access both.
+In typical use, some monadic operations that are overloaded in type classes have type information available for {tech key:="synthesis"}[instance synthesis], while others do not.
+For example, the argument passed to {name MonadState.set}`set` determines the type of the state to be used, while {name MonadState.get}`get` takes no such argument.
+The type information present in applications of {name MonadState.set}`set` can be used to pick the correct instance when multiple states are available, which suggests that the type of the mutable state should be an input parameter or {tech}[semi-output parameter] so that it can be used to select instances.
+The lack of type information present in uses of {name MonadState.get}`get`, on the other hand, suggests that the type of the mutable state should be an {tech}[output parameter] in {lean}`MonadState`, so type class synthesis determines the state's type from the monad itself.
+
+This dichotomy is solved by having two versions of many of the effect type classes.
+The version with a semi-output parameter has the suffix `-Of`, and its operations take types explicitly as needed.
+Examples include {name}`MonadStateOf`, {name}`MonadReaderOf`, and {name}`MonadExceptOf`.
+The operations with explicit type parameters have names ending in `-The`, such as {name}`getThe`, {name}`readThe`, and {name}`tryCatchThe`.
+The name of the version with an output parameter is undecorated.
+The standard library exports a mix of operations from the `-Of` and undecorated versions of each type class, based on what has good inference behavior in typical use cases.
+
+:::table (header := true)
+  * ignored
+   * Operation
+   * From Class
+   * Notes
+  * ignored
+   * {name}`get`
+   * {name}`MonadState`
+   * Output parameter improves type inference
+  * ignored
+   * {name}`set`
+   * {name}`MonadStateOf`
+   * Semi-output parameter uses type information from {name}`set`'s argument
+  * ignored
+   * {name}`modify`
+   * {name}`MonadState`
+   * Output parameter is needed to allow functions without annotations
+  * ignored
+   * {name}`modifyGet`
+   * {name}`MonadState`
+   * Output parameter is needed to allow functions without annotations
+  * ignored
+   * {name}`read`
+   * {name}`MonadReader`
+   * Output parameter is needed due to lack of type information from arguments
+  * ignored
+   * {name}`readThe`
+   * {name}`MonadReaderOf`
+   * Semi-output parameter uses the provided type to guide synthesis
+  * ignored
+   * {name}`withReader`
+   * {name}`MonadWithReader`
+   * Output parameter avoids the need for type annotations on the function
+  * ignored
+   * {name}`withTheReader`
+   * {name}`MonadWithReaderOf`
+   * Semi-output parameter uses provided type to guide synthesis
+  * ignored
+   * {name}`throw`
+   * {name}`MonadExcept`
+   * Output parameter enables the use of constructor dot notation for the exception
+  * ignored
+   * {name}`throwThe`
+   * {name}`MonadExceptOf`
+   * Semi-output parameter uses provided type to guide synthesis
+  * ignored
+   * {name}`tryCatch`
+   * {name}`MonadExcept`
+   * Output parameter enables the use of constructor dot notation for the exception
+  * ignored
+   * {name}`tryCatchThe`
+   * {name}`MonadExceptOf`
+   * Semi-output parameter uses provided type to guide synthesis
+:::
+
+```lean (show := false)
+example : @get = @MonadState.get := by rfl
+example : @set = @MonadStateOf.set := by rfl
+example (f : σ → σ) : @modify σ m inst f = @MonadState.modifyGet σ m inst PUnit fun (s : σ) => (PUnit.unit, f s) := by rfl
+example : @modifyGet = @MonadState.modifyGet := by rfl
+example : @read = @MonadReader.read := by rfl
+example : @readThe = @MonadReaderOf.read := by rfl
+example : @withReader = @MonadWithReader.withReader := by rfl
+example : @withTheReader = @MonadWithReaderOf.withReader := by rfl
+example : @throw = @MonadExcept.throw := by rfl
+example : @throwThe = @MonadExceptOf.throw := by rfl
+example : @tryCatch = @MonadExcept.tryCatch := by rfl
+example : @tryCatchThe = @MonadExceptOf.tryCatch := by rfl
+```
+
+:::example "State Types"
+The state monad {name}`M` has two separate states: a {lean}`Nat` and a {lean}`String`.
+```lean
+abbrev M := StateT Nat (StateM String)
+```
+
+Because {name}`get` is an alias for {name}`MonadState.get`, the state type is an output parameter.
+This means that Lean selects a state type automatically, in this case the one from the outermost monad transformer:
+```lean (name := getM)
+#check (get : M _)
+```
+```leanOutput getM
+get : M Nat
+```
+
+Only the outermost may be used, because the type of the state is an output parameter.
+```lean (name := getMStr) (error := true)
+#check (get : M String)
+```
+```leanOutput getMStr
+failed to synthesize
+  MonadState String M
+Additional diagnostic information may be available using the `set_option diagnostics true` command.
+```
+
+Providing the state type explicitly using {name}`getThe` from {name}`MonadStateOf` allows both states to be read.
+```lean (name := getTheM)
+#check ((getThe String, getThe Nat) : M String × M Nat)
+```
+```leanOutput getTheM
+(getThe String, getThe Nat) : M String × M Nat
+```
+
+Setting a state works for either type, because the state type is a {tech}[semi-output parameter] on {name}`MonadStateOf`.
+```lean (name := setNat)
+#check (set 4 : M Unit)
+```
+```leanOutput setNat
+set 4 : M PUnit
+```
+
+```lean (name := setStr)
+#check (set "Four" : M Unit)
+```
+```leanOutput setStr
+set "Four" : M PUnit
+```
+
+:::
+
+
+# Monad Transformers
+
+A {deftech}_monad transformer_ is a function that, when provided with a monad, gives back a new monad.
+Typically, this new monad has all the effects of the original monad along with some additional ones.
+
+```lean (show := false)
+variable {α : Type u} (T : (Type u → Type v) → Type u → Type w) (m : Type u → Type v)
+
+```
+A monad transformer consists of the following:
+ * A function {lean}`T` that constructs the new monad's type from an existing monad
+ * A `run` function that adapts a {lean}`T m α` into some variant of {lean}`m`, often requiring additional parameters and returning a more specific type under {lean}`m`
+ * An instance of {lean}`[Monad m] → Monad (T m)` that allows the transformed monad to be used as a monad
+ * An instance of {lean}`MonadLift` that allows the original monad's code to be used in the transformed monad
+ * If possible, an instance of {lean}`MonadControl m (T m)` that allows actions from the transformed monad to be used in the original monad
+
+Typically, a monad transformer also provides instances of one or more type classes that describe the effects that it introduces.
+The transformer's {name}`Monad` and {name}`MonadLift` instances make it practical to write code in the transformed monad, while the type class instances allow the transformed monad to be used with polymorphic functions.
+
+::::keepEnv
+```lean (show := false)
+universe u v
+variable {m : Type u → Type v} {α : Type u}
+```
+:::example "The Identity Monad Transformer "
+The identity monad transformer neither adds nor removes capabilities to the transformed monad.
+Its definition is the identity function, suitably specialized:
+```lean
+def IdT (m : Type u → Type v) : Type u → Type v := m
+```
+Similarly, the {name IdT.run}`run` function requires no additional arguments and just returns an {lean}`m α`:
+```lean
+def IdT.run (act : IdT m α) : m α := act
+```
+
+The monad instance relies on the monad instance for the transformed monad, selecting it via {tech}[type ascriptions]:
+```lean
+instance [Monad m] : Monad (IdT m) where
+  pure x := (pure x : m _)
+  bind x f := (x >>= f : m _)
+```
+
+Because {lean}`IdT m` is definitionally equal to {lean}`m`, the {lean}`MonadLift m (IdT m)` instance doesn't need to modify the action being lifted:
+```lean
+instance : MonadLift m (IdT m) where
+  monadLift x := x
+```
+
+The {lean}`MonadControl` instance is similarly simple.
+```lean
+instance [Monad m] : MonadControl m (IdT m) where
+  stM α := α
+  liftWith f := f (fun x => Id.run <| pure x)
+  restoreM v := v
+```
+
+:::
+::::
+
+The Lean standard library provides transformer versions of many different monads, including {name}`ReaderT`, {name}`ExceptT`, and {name}`StateT`, along with variants using other representations such as {name}`StateCpsT`, {name StateRefT'}`StateRefT`, and {name}`ExceptCpsT`.
+Additionally, the {name}`EStateM` monad is equivalent to combining {name}`ExceptT` and {name}`StateT`, but it can use a more specialized representation to improve performance.
+
+{include 0 Monads.Zoo.Id}
+
+{include 0 Monads.Zoo.State}
+
+{include 0 Monads.Zoo.Reader}
+
+{include 0 Monads.Zoo.Option}
+
+{include 0 Monads.Zoo.Except}
+
+{include 0 Monads.Zoo.Combined}
