Manual/Monads/Zoo/Combined.lean
@@ -1,0 +1,98 @@
+/-
+Copyright (c) 2024 Lean FRO LLC. All rights reserved.
+Released under Apache 2.0 license as described in the file LICENSE.
+Author: David Thrane Christiansen
+-/
+
+import VersoManual
+
+import Manual.Meta
+
+import Lean.Parser.Command
+
+open Manual
+
+open Verso.Genre
+open Verso.Genre.Manual
+
+set_option pp.rawOnError true
+
+set_option linter.unusedVariables false
+
+#doc (Manual) "Combined Error and State Monads" =>
+
+```lean (show := false)
+variable (ε : Type u) (σ σ' : Type u) (α : Type u)
+```
+
+The {name}`EStateM` monad has both exceptions and mutable state.
+{lean}`EStateM ε σ α` is logically equivalent to {lean}`ExceptT ε (StateM σ) α`.
+While {lean}`ExceptT ε (StateM σ)` evaluates to the type {lean}`σ → Except ε α × σ`, the type {lean}`EStateM ε σ α` evaluates to {lean}`σ → EStateM.Result ε σ α`.
+{name}`EStateM.Result` is an inductive type that's very similar to {name}`Except`, except both constructors have an additional field for the state.
+In compiled code, this representation removes one level of indirection from each monadic bind.
+
+```lean (show := false)
+/-- info: σ → Except ε α × σ -/
+#guard_msgs in
+#reduce (types := true) ExceptT ε (StateM σ) α
+
+/-- info: σ → EStateM.Result ε σ α -/
+#guard_msgs in
+#reduce (types := true) EStateM ε σ α
+```
+
+{docstring EStateM}
+
+{docstring EStateM.Result}
+
+{docstring EStateM.run}
+
+{docstring EStateM.run'}
+
+{docstring EStateM.adaptExcept}
+
+{docstring EStateM.fromStateM}
+
+# State Rollback
+
+Composing {name}`StateT` and {name}`ExceptT` in different orders causes exceptions to interact differently with state.
+In one ordering, state changes are rolled back when exceptions are caught; in the other, they persist.
+The latter option matches the semantics of most imperative programming languages, but the former is very useful for search-based problems.
+Often, some but not all state should be rolled back; this can be achieved by “sandwiching” {name}`ExceptT` between two separate uses of {name}`StateT`.
+
+To avoid yet another layer of indirection via the use of {lean}`StateT σ (EStateM ε σ') α`, {name}`EStateM` offers the {name}`EStateM.Backtrackable` {tech}[type class].
+This class specifies some part of the state that can be saved and restored.
+{name}`EStateM` then arranges for the saving and restoring to take place around error handling.
+
+{docstring EStateM.Backtrackable}
+
+There is a universally-applicable instance of {name EStateM.Backtrackable}`Backtrackable` that neither saves nor restores anything.
+Because instance synthesis chooses the most recent instance first, the universal instance is used only if no other instance has been defined.
+
+{docstring EStateM.nonBacktrackable}
+
+# Implementations
+
+These functions are typically not called directly, but rather are accessed through their corresponding type classes.
+
+{docstring EStateM.map}
+
+{docstring EStateM.pure}
+
+{docstring EStateM.bind}
+
+{docstring EStateM.orElse}
+
+{docstring EStateM.orElse'}
+
+{docstring EStateM.seqRight}
+
+{docstring EStateM.tryCatch}
+
+{docstring EStateM.throw}
+
+{docstring EStateM.get}
+
+{docstring EStateM.set}
+
+{docstring EStateM.modifyGet}
