Manual/Monads/Zoo/Except.lean
@@ -1,0 +1,127 @@
+/-
+Copyright (c) 2024 Lean FRO LLC. All rights reserved.
+Released under Apache 2.0 license as described in the file LICENSE.
+Author: David Thrane Christiansen
+-/
+
+import VersoManual
+
+import Manual.Meta
+
+import Lean.Parser.Command
+
+open Manual
+
+open Verso.Genre
+open Verso.Genre.Manual
+
+set_option pp.rawOnError true
+
+set_option linter.unusedVariables false
+
+#doc (Manual) "Exceptions" =>
+%%%
+tag := "exception-monads"
+%%%
+
+Exception monads describe computations that terminate early (fail).
+Failing computations provide their caller with an _exception_ value that describes _why_ they failed.
+In other words, computations either return a value or an exception.
+The inductive type {name}`Except` captures this pattern, and is itself a monad.
+
+# Exceptions
+
+{docstring Except}
+
+{docstring Except.pure}
+
+{docstring Except.bind}
+
+{docstring Except.map}
+
+{docstring Except.mapError}
+
+{docstring Except.tryCatch}
+
+{docstring Except.orElseLazy}
+
+{docstring Except.isOk}
+
+{docstring Except.toOption}
+
+{docstring Except.toBool}
+
+
+# Type Class
+
+{docstring MonadExcept}
+
+{docstring MonadExcept.ofExcept}
+
+{docstring MonadExcept.orElse}
+
+{docstring MonadExcept.orelse'}
+
+{docstring MonadExceptOf}
+
+{docstring throwThe}
+
+{docstring tryCatchThe}
+
+# “Finally” Computations
+
+{docstring MonadFinally}
+
+# Transformer
+
+{docstring ExceptT}
+
+{docstring ExceptT.lift}
+
+{docstring ExceptT.run}
+
+{docstring ExceptT.pure}
+
+{docstring ExceptT.bind}
+
+{docstring ExceptT.bindCont}
+
+{docstring ExceptT.tryCatch}
+
+{docstring ExceptT.mk}
+
+{docstring ExceptT.map}
+
+{docstring ExceptT.adapt}
+
+
+# Exception Monads in Continuation Passing Style
+
+```lean (show := false)
+universe u
+variable (α : Type u)
+variable (ε : Type u)
+variable {m : Type u → Type v}
+```
+
+Continuation-passing-style exception monads represent potentially-failing computations as functions that take success and failure continuations, both of which return the same type, returning that type.
+They must work for _any_ return type.
+An example of such a type is {lean}`(β : Type u) → (α → β) → (ε → β) → β`.
+{lean}`ExceptCpsT` is a transformer that can be applied to any monad, so {lean}`ExceptCpsT ε m α` is actually defined as {lean}`(β : Type u) → (α → m β) → (ε → m β) → m β`.
+Exception monads in continuation passing style have different performance characteristics than {name}`Except`-based state monads; for some applications, it may be worth benchmarking them.
+
+```lean (show := false)
+/-- info: (β : Type u) → (α → m β) → (ε → m β) → m β -/
+#guard_msgs in
+#reduce (types := true) ExceptCpsT ε m α
+```
+
+{docstring ExceptCpsT}
+
+{docstring ExceptCpsT.runCatch}
+
+{docstring ExceptCpsT.runK}
+
+{docstring ExceptCpsT.run}
+
+{docstring ExceptCpsT.lift}
