Manual/Monads/Zoo/Id.lean
@@ -1,0 +1,56 @@
+/-
+Copyright (c) 2024 Lean FRO LLC. All rights reserved.
+Released under Apache 2.0 license as described in the file LICENSE.
+Author: David Thrane Christiansen
+-/
+
+import VersoManual
+
+import Manual.Meta
+
+import Lean.Parser.Command
+
+open Manual
+
+open Verso.Genre
+open Verso.Genre.Manual
+
+set_option pp.rawOnError true
+
+set_option linter.unusedVariables false
+
+#doc (Manual) "Identity" =>
+
+The identity monad {name}`Id` has no effects whatsoever.
+Both {name}`Id` and the corresponding implementation of {name}`pure` are the identity function, and {name}`bind` is reversed function application.
+The identity monad has two primary use cases:
+ 1. It can be the type of a {keywordOf Lean.Parser.Term.do}`do` block that implements a pure function with local effects.
+ 2. It can be placed at the bottom of a stack of monad transformers.
+
+```lean (show := false)
+-- Verify claims
+example : Id = id := rfl
+example : Id.run (α := α) = id := rfl
+example : (pure (f := Id)) = (id : α → α) := rfl
+example : (bind (m := Id)) = (fun (x : α) (f : α → Id β) => f x) := rfl
+```
+
+{docstring Id}
+
+{docstring Id.run}
+
+:::example "Local Effects with the Identity Monad"
+This code block implements a countdown procedure by using simulated local mutability in the identity monad.
+```lean (name := idDo)
+#eval Id.run do
+  let mut xs := []
+  for x in [0:10] do
+    xs := x :: xs
+  pure xs
+```
+```leanOutput idDo
+[9, 8, 7, 6, 5, 4, 3, 2, 1, 0]
+```
+:::
+
+{docstring Id.hasBind}
