Manual/Monads/Zoo/Option.lean
@@ -1,0 +1,48 @@
+/-
+Copyright (c) 2024 Lean FRO LLC. All rights reserved.
+Released under Apache 2.0 license as described in the file LICENSE.
+Author: David Thrane Christiansen
+-/
+
+import VersoManual
+
+import Manual.Meta
+
+import Lean.Parser.Command
+
+open Manual
+
+open Verso.Genre
+open Verso.Genre.Manual
+
+set_option pp.rawOnError true
+
+set_option linter.unusedVariables false
+
+#doc (Manual) "Option" =>
+%%%
+tag := "option-monad"
+%%%
+
+Ordinarily, {lean}`Option` is thought of as data, similarly to a nullable type.
+It can also be considered as a monad, and thus a way of performing computations.
+The {lean}`Option` monad and its transformer {lean}`OptionT` can be understood as describing computations that may terminate early, discarding the results.
+Callers can check for early termination and invoke a fallback if desired using {name}`OrElse.orElse` or by treating it as a {lean}`MonadExcept Unit`.
+
+{docstring OptionT}
+
+{docstring OptionT.run}
+
+{docstring OptionT.lift}
+
+{docstring OptionT.mk}
+
+{docstring OptionT.pure}
+
+{docstring OptionT.bind}
+
+{docstring OptionT.fail}
+
+{docstring OptionT.orElse}
+
+{docstring OptionT.tryCatch}
