Manual/Monads/Zoo/Reader.lean
@@ -1,0 +1,53 @@
+/-
+Copyright (c) 2024 Lean FRO LLC. All rights reserved.
+Released under Apache 2.0 license as described in the file LICENSE.
+Author: David Thrane Christiansen
+-/
+
+import VersoManual
+
+import Manual.Meta
+
+import Lean.Parser.Command
+
+open Manual
+
+open Verso.Genre
+open Verso.Genre.Manual
+
+set_option pp.rawOnError true
+
+set_option linter.unusedVariables false
+
+#doc (Manual) "Reader" =>
+
+
+{docstring MonadReader}
+
+{docstring MonadReaderOf}
+
+{docstring readThe}
+
+{docstring MonadWithReader}
+
+{docstring MonadWithReaderOf}
+
+{docstring withTheReader}
+
+{docstring ReaderT}
+
+{docstring ReaderM}
+
+{docstring ReaderT.adapt}
+
+{docstring ReaderT.read}
+
+{docstring ReaderT.run}
+
+{docstring ReaderT.orElse}
+
+{docstring ReaderT.bind}
+
+{docstring ReaderT.failure}
+
+{docstring ReaderT.pure}
