Manual/Monads/Zoo/State.lean
@@ -1,0 +1,150 @@
+/-
+Copyright (c) 2024 Lean FRO LLC. All rights reserved.
+Released under Apache 2.0 license as described in the file LICENSE.
+Author: David Thrane Christiansen
+-/
+
+import VersoManual
+
+import Manual.Meta
+
+import Lean.Parser.Command
+
+open Manual
+
+open Verso.Genre
+open Verso.Genre.Manual
+
+set_option pp.rawOnError true
+
+set_option linter.unusedVariables false
+
+#doc (Manual) "State" =>
+%%%
+tag := "state-monads"
+%%%
+
+{tech}[State monads] provide access to a mutable value.
+The underlying implementation may a tuple to simulate mutability, or it may use something like {name}`ST.Ref` to ensure mutation.
+Even those implementations that use a tuple may in fact use mutation at run-time due to Lean's use of mutation when there are unique references to values, but this requires a programming style that prefers {name}`modify` and {name}`modifyGet` over {name}`get` and {name}`set`.
+
+# General State API
+
+{docstring MonadState}
+
+{docstring get}
+
+{docstring modify}
+
+{docstring modifyGet}
+
+{docstring getModify}
+
+{docstring MonadStateOf}
+
+{docstring getThe}
+
+{docstring modifyThe}
+
+{docstring modifyGetThe}
+
+# Tuple-Based State Monads
+
+```lean (show := false)
+variable {α σ : Type u}
+```
+
+The tuple-based state monads represent a computation with states that have type {lean}`σ` yielding values of type {lean}`α` as functions that take a starting state and yield a value paired with a final state, e.g. {lean}`σ → α × σ`.
+The {name}`Monad` operations thread the state correctly through the computation.
+
+{docstring StateM}
+
+{docstring StateT}
+
+{docstring StateT.run}
+
+{docstring StateT.get}
+
+{docstring StateT.set}
+
+{docstring StateT.orElse}
+
+{docstring StateT.failure}
+
+{docstring StateT.run'}
+
+{docstring StateT.bind}
+
+{docstring StateT.modifyGet}
+
+{docstring StateT.lift}
+
+{docstring StateT.map}
+
+{docstring StateT.pure}
+
+# State Monads in Continuation Passing Style
+
+Continuation-passing-style state monads represent stateful computations as functions that, for any type whatsoever, take an initial state and a continuation (modeled as a function) that accepts a value and an updated state.
+An example of such a type is {lean}`(δ : Type u) → σ → (α → σ → δ) → δ`, though {lean}`StateCpsT` is a transformer that can be applied to any monad.
+State monads in continuation passing style have different performance characteristics than tuple-based state monads; for some applications, it may be worth benchmarking them.
+
+
+```lean (show := false)
+/-- info: (δ : Type u) → σ → (α → σ → Id δ) → δ -/
+#guard_msgs in
+#reduce (types := true) StateCpsT σ Id α
+```
+{docstring StateCpsT}
+
+{docstring StateCpsT.lift}
+
+{docstring StateCpsT.runK}
+
+{docstring StateCpsT.run'}
+
+{docstring StateCpsT.run}
+
+# State Monads from Mutable References
+
+```lean (show := false)
+variable {m : Type → Type} {σ ω : Type} [STWorld σ m]
+```
+
+The monad {lean}`StateRefT σ m` is a specialized state monad transformer that can be used when {lean}`m` is a monad to which {name}`ST` computations can be lifted.
+It implements the operations of {name}`MonadState` using an {name}`ST.Ref`, rather than pure functions.
+This ensures that mutation is actually used at run time.
+
+{name}`ST` and {name}`EST` require a phantom type parameter that's used together with {name}`runST`'s polymorphic function argument to encapsulate mutability.
+Rather than require this as a parameter to the transformer, an auxiliary type class {name}`STWorld` is used to propagate it directly from {lean}`m`.
+
+The transformer itself is defined as a {ref "syntax-ext"}[syntax extension] and an {ref "elaborators"}[elaborator], rather than an ordinary function.
+This is because {name}`STWorld` has no methods: it exists only to propagate information from the inner monad to the transformed monad.
+Nonetheless, its instances are terms; keeping them around could lead to unnecessarily large types.
+
+{docstring STWorld}
+
+:::syntax term
+The syntax for {lean}`StateRefT σ m` accepts two arguments:
+
+```grammar
+StateRefT $_ $_
+```
+
+Its elaborator synthesizes an instance of {lean}`STWorld ω m` to ensure that {lean}`m` supports mutable references.
+Having discovered the value of {lean}`ω`, it then produces the term {lean}`StateRefT' ω σ m`, discarding the synthesized instance.
+:::
+
+{docstring StateRefT'}
+
+{docstring StateRefT'.get}
+
+{docstring StateRefT'.set}
+
+{docstring StateRefT'.modifyGet}
+
+{docstring StateRefT'.run}
+
+{docstring StateRefT'.run'}
+
+{docstring StateRefT'.lift}
