Manual/NotationsMacros/SyntaxDef.lean
@@ -20,6 +20,9 @@ set_option pp.rawOnError true
 set_option linter.unusedVariables false
 
 #doc (Manual) "Defining New Syntax" =>
+%%%
+tag := "syntax-ext"
+%%%
 
 Lean's uniform representation of syntax is very general and flexible.
 This means that extensions to Lean's parser do not require extensions to the representation of parsed syntax.
