Manual/Terms.lean
@@ -30,6 +30,5 @@ This chapter will describe Lean's term language, including the following feature
  * Pattern matching, including `match`, `let`, `if let`, `matches`, `nomatch`, `nofun`
  * Do-notation, including `let mut`, `for`, `while`, `repeat`, `break`, `return`
  * {deftech}_Holes_ and {deftech}_named holes_
-
-
+ * {deftech}_Type ascription_ syntax
 :::
